add a few machine-generated examples for an article

Docs/ContextualEmbedding/CEExtrinsic.lean
@@ -1,5 +1,9 @@
 namespace ContextualEmbedding.CEExtrinsic
 
+/-
+derived from CE.lean, but using extrinsic typing instead of intrinsic typing
+-/
+
 inductive Ty : Type
   | Unit : Ty
   | Fun : Ty -> Ty -> Ty
@@ -10,7 +14,7 @@ infixr:90 " :-> " => Fun
 
 inductive Ctx : Type
   | Empty : Ctx
-  | Snoc  : Ctx -> Ty -> Ctx
+  | Snoc : Ctx -> Ty -> Ctx
 deriving Repr, DecidableEq
 
 infixl:90 " :/: " => Ctx.Snoc
@@ -27,18 +31,18 @@ inductive Lookup : Ctx -> Index -> Ty -> Type where
 deriving Repr
 
 inductive STLC : Type where
-  | Var    : Index -> STLC
-  | Star   : STLC
+  | Var : Index -> STLC
+  | Star : STLC
   | Lambda : Ty -> STLC -> STLC
-  | Apply  : STLC -> STLC -> STLC
+  | Apply : STLC -> STLC -> STLC
 deriving Repr, DecidableEq
 open STLC
 
 inductive HasType : Ctx -> STLC -> Ty -> Type where
-  | Var    : Lookup ts i t -> HasType ts (Var i) t
-  | Star   : HasType ts Star Unit
+  | Var : Lookup ts i t -> HasType ts (Var i) t
+  | Star : HasType ts Star Unit
   | Lambda : HasType (ts :/: t1) e t2 -> HasType ts (Lambda t1 e) (t1 :-> t2)
-  | Apply  : HasType ts e1 (t1 :-> t2) -> HasType ts e2 t1 -> HasType ts (Apply e1 e2) t2
+  | Apply : HasType ts e1 (t1 :-> t2) -> HasType ts e2 t1 -> HasType ts (Apply e1 e2) t2
 deriving Repr
 
 inductive ProxyTop : Ctx -> Ty -> Type where
@@ -62,38 +66,40 @@ def reifyWith : ReifyIndex ts ts' t -> ProxyTop ts t -> Index
   | Refl, PTop => Top
   | Snoc instRec, i => Pop (reifyWith instRec i)
 
-def reify {ts ts' : Ctx} {t : Ty} [inst : ReifyIndex ts ts' t] : ProxyTop ts t -> Index :=
-  reifyWith inst
-
 def reifyLookupWith : (inst : ReifyIndex ts ts' t) -> (i : ProxyTop ts t) -> Lookup ts' (reifyWith inst i) t
   | Refl, PTop => Lookup.Top
   | Snoc instRec, i => Lookup.Pop (reifyLookupWith instRec i)
 
-def reifyLookup {ts ts' : Ctx} {t : Ty} [inst : ReifyIndex ts ts' t] (i : ProxyTop ts t) :
-    Lookup ts' (reify (inst := inst) i) t :=
-  reifyLookupWith inst i
-
-inductive STLCCtx : Ctx -> Ty -> Type where
-  | CVar [inst : ReifyIndex ts ts' t] : ProxyTop ts t -> STLCCtx ts' t
-  | CStar : STLCCtx ts Unit
-  | CLam : (ProxyTop (ts :/: a) a -> STLCCtx (ts :/: a) b) -> STLCCtx ts (a :-> b)
-  | CApp : STLCCtx ts (a :-> b) -> STLCCtx ts a -> STLCCtx ts b
+inductive STLCCtx : Type where
+  | CVar {ts ts' : Ctx} {t : Ty} [inst : ReifyIndex ts ts' t] : ProxyTop ts t -> STLCCtx
+  | CStar : STLCCtx
+  | CLam {ts : Ctx} (a : Ty) : (ProxyTop (ts :/: a) a -> STLCCtx) -> STLCCtx
+  | CApp : STLCCtx -> STLCCtx -> STLCCtx
 open STLCCtx
 
-def unembed : STLCCtx ts t -> STLC
-  | CStar      => STLC.Star
+inductive CtxHasType : Ctx -> STLCCtx -> Ty -> Type where
+  | CVar {ts ts' : Ctx} {t : Ty} (inst : ReifyIndex ts ts' t) (i : ProxyTop ts t) :
+      CtxHasType ts' (CVar (inst := inst) i) t
+  | CStar : CtxHasType ts CStar Unit
+  | CLam {ts : Ctx} {a b : Ty} {body : ProxyTop (ts :/: a) a -> STLCCtx} :
+      ((i : ProxyTop (ts :/: a) a) -> CtxHasType (ts :/: a) (body i) b) ->
+        CtxHasType ts (CLam a body) (a :-> b)
+  | CApp : CtxHasType ts e1 (a :-> b) -> CtxHasType ts e2 a -> CtxHasType ts (CApp e1 e2) b
+
+def unembed : STLCCtx -> STLC
+  | CStar => STLC.Star
   | @CVar _ _ _ inst i => STLC.Var (reifyWith inst i)
-  | @CLam _ a _ e => STLC.Lambda a (unembed (e PTop))
+  | @CLam _ a body => STLC.Lambda a (unembed (body PTop))
   | CApp e1 e2 => STLC.Apply (unembed e1) (unembed e2)
 
-def unembedTyped : (e : STLCCtx ts t) -> HasType ts (unembed e) t
-  | CStar      => HasType.Star
-  | @CVar _ _ _ inst i => HasType.Var (reifyLookupWith inst i)
-  | CLam e     => HasType.Lambda (unembedTyped (e PTop))
-  | CApp e1 e2 => HasType.Apply (unembedTyped e1) (unembedTyped e2)
+def unembedTyped : CtxHasType ts e t -> HasType ts (unembed e) t
+  | CtxHasType.CStar => HasType.Star
+  | @CtxHasType.CVar _ _ _ inst i => HasType.Var (reifyLookupWith inst i)
+  | CtxHasType.CLam bodyTyped => HasType.Lambda (unembedTyped (bodyTyped PTop))
+  | CtxHasType.CApp e1 e2 => HasType.Apply (unembedTyped e1) (unembedTyped e2)
 
-inductive ProxyVar ts' t where
-  | PVar [inst : ReifyIndex ts ts' t] : ProxyTop ts t -> ProxyVar ts' t
+inductive ProxyVar (ts' : Ctx) (t : Ty) where
+  | PVar {ts : Ctx} [inst : ReifyIndex ts ts' t] : ProxyTop ts t -> ProxyVar ts' t
 deriving Repr
 open ProxyVar
 
@@ -102,24 +108,30 @@ def weakenPVar : ProxyVar ts' t -> ProxyVar (ts' :/: t') t
 
 def varTop : ProxyVar (ts :/: t) t := PVar (inst := Refl) (@PTop ts t)
 
-def fromVar : ProxyVar ts' t -> STLCCtx ts' t
+def fromVar : ProxyVar ts' t -> STLCCtx
   | @PVar _ _ _ inst i => CVar (inst := inst) i
 
+def fromVarTyped : (v : ProxyVar ts t) -> CtxHasType ts (fromVar v) t
+  | @PVar _ _ _ inst i => CtxHasType.CVar inst i
+
 def fromLookup : Lookup ts i t -> ProxyVar ts t
-  | Lookup.Top   => varTop
+  | Lookup.Top => varTop
   | Lookup.Pop h => weakenPVar (fromLookup h)
 
-def toCVar : Lookup ts i t -> STLCCtx ts t :=
-  fun i => fromVar (fromLookup i)
+def contextualise : HasType ts e t -> STLCCtx
+  | @HasType.Var _ _ _ h => fromVar (fromLookup h)
+  | @HasType.Star _ => CStar
+  | @HasType.Lambda ts t1 _ _ h => @CLam ts t1 (fun _ => contextualise h)
+  | @HasType.Apply _ _ _ _ _ h1 h2 => CApp (contextualise h1) (contextualise h2)
 
-def contextualise : HasType ts e t -> STLCCtx ts t
-  | HasType.Var i => toCVar i
-  | HasType.Lambda e => CLam (fun _ => contextualise e)
-  | HasType.Apply e1 e2 => CApp (contextualise e1) (contextualise e2)
-  | HasType.Star => CStar
+def contextualiseTyped : (h : HasType ts e t) -> CtxHasType ts (contextualise h) t
+  | @HasType.Var _ _ _ h => fromVarTyped (fromLookup h)
+  | @HasType.Star _ => CtxHasType.CStar
+  | @HasType.Lambda _ _ _ _ h => CtxHasType.CLam (fun _ => contextualiseTyped h)
+  | @HasType.Apply _ _ _ _ _ h1 h2 => CtxHasType.CApp (contextualiseTyped h1) (contextualiseTyped h2)
 
-theorem indexIsoL (i : Lookup ts idx t)
-  : reifyWith (fromLookup i).2 (fromLookup i).3 = idx := by
+theorem indexIsoL (i : Lookup ts idx t) :
+    reifyWith (fromLookup i).2 (fromLookup i).3 = idx := by
   induction i with
   | Top => rfl
   | Pop i' ih =>
@@ -137,94 +149,144 @@ theorem indexIsoR (inst : ReifyIndex ts ts' t) (i : ProxyTop ts t) :
         = weakenPVar (PVar (inst := instRec) i)
       rw [ih]
 
-theorem isoL {h : HasType ts e t}
-  : unembed (contextualise h) = e := by
+theorem isoL {h : HasType ts e t} :
+    unembed (contextualise h) = e := by
   induction h with
   | Star => rfl
-  | Apply e1 e2 ih1 ih2 => simp [contextualise, unembed, ih1, ih2]
-  | Lambda e ih => simp [contextualise, unembed, ih]
-  | Var i => simp [contextualise, toCVar, fromVar, unembed, indexIsoL]
+  | Apply _ _ ih1 ih2 => simp [contextualise, unembed, ih1, ih2]
+  | Lambda _ ih => simp [contextualise, unembed, ih]
+  | Var i => simp [contextualise, fromVar, unembed, indexIsoL]
 
-theorem isoL' {h : HasType ts e t}
-  : unembed (contextualise h) = e := by
+theorem isoL' {h : HasType ts e t} :
+    unembed (contextualise h) = e := by
   induction h
     <;> simp [contextualise, unembed, *]
-  case Var => simp [toCVar, fromVar, unembed, indexIsoL]
+  case Var => simp [fromVar, unembed, indexIsoL]
 
-theorem isoR {e : STLCCtx ts t}
-  : contextualise (unembedTyped e) = e := by
-  induction e with
+theorem isoR {h : CtxHasType ts e t} :
+    contextualise (unembedTyped h) = e := by
+  induction h with
   | CStar => rfl
-  | CApp e1 e2 ih1 ih2 => simp [unembedTyped, contextualise, ih1, ih2]
-  | CVar => simp [unembedTyped, contextualise, toCVar, indexIsoR]
-            rfl
-  | CLam f ih =>
+  | CApp _ _ ih1 ih2 => simp [unembedTyped, contextualise, ih1, ih2]
+  | CVar inst i =>
+      change fromVar (fromLookup (reifyLookupWith inst i)) = CVar (inst := inst) i
+      rw [indexIsoR inst i]
+      rfl
+  | CLam bodyTyped ih =>
       simp [unembedTyped, contextualise, unembed]
       funext x
-      simp [ih]
       cases x
-      rfl
+      exact ih PTop
 
-theorem isoR' {e : STLCCtx ts t}
-  : contextualise (unembedTyped e) = e := by
-  induction e
+theorem isoR' {h : CtxHasType ts e t} :
+    contextualise (unembedTyped h) = e := by
+  induction h
     <;> try (simp [unembedTyped, contextualise, unembed, *])
     <;> try (repeat' (funext p; cases p)
              <;> simp [*])
-  case CVar => simp [toCVar, indexIsoR]
-               rfl
+  case CVar inst i =>
+    change fromVar (fromLookup (reifyLookupWith inst i)) = CVar (inst := inst) i
+    rw [indexIsoR inst i]
+    rfl
 
-def showSTLCCtx : STLCCtx ts t -> String
+def showSTLCCtx : STLCCtx -> String
   | @CVar _ _ _ inst i => "CVar " ++ reprStr i ++ "[reified = " ++ reprStr (reifyWith inst i) ++ "]"
-  | CStar  => "CStar"
-  | CLam f => "CLam (\\<ProxyTop> -> " ++ showSTLCCtx (f PTop) ++ ")"
+  | CStar => "CStar"
+  | @CLam _ _ body => "CLam (\\<ProxyTop> -> " ++ showSTLCCtx (body PTop) ++ ")"
   | CApp f x => "CApp (" ++ showSTLCCtx f ++ ") (" ++ showSTLCCtx x ++ ")"
 
-def idSTLC : STLCCtx ts (a :-> a)
-  := CLam (fun x => CVar x)
-def idSTLC' := @idSTLC Ctx.Empty Unit
+def idSTLC (ts : Ctx) (a : Ty) : STLCCtx :=
+  @CLam ts a (fun x => @CVar (ts :/: a) (ts :/: a) a Refl x)
+
+def idSTLCTyped (ts : Ctx) (a : Ty) : CtxHasType ts (idSTLC ts a) (a :-> a) :=
+  CtxHasType.CLam (fun x => CtxHasType.CVar Refl x)
+
+def idSTLC' : STLCCtx := idSTLC Ctx.Empty Unit
+
+def idSTLC'Typed : CtxHasType Ctx.Empty idSTLC' (Unit :-> Unit) :=
+  idSTLCTyped Ctx.Empty Unit
 
 #check idSTLC
 #eval showSTLCCtx idSTLC'
 #eval unembed idSTLC'
-#eval showSTLCCtx (contextualise (unembedTyped idSTLC'))
-#eval unembed (contextualise (unembedTyped idSTLC'))
+#eval showSTLCCtx (contextualise (unembedTyped idSTLC'Typed))
+#eval unembed (contextualise (unembedTyped idSTLC'Typed))
 
-def const : STLCCtx ts (a :-> b :-> a)
-  := CLam (fun x => CLam (fun _ => CVar x))
-def const' := @const Ctx.Empty Unit Unit
+def const (ts : Ctx) (a b : Ty) : STLCCtx :=
+  @CLam ts a (fun x =>
+    @CLam (ts :/: a) b (fun _ =>
+      @CVar (ts :/: a) ((ts :/: a) :/: b) a (Snoc Refl) x))
+
+def constTyped (ts : Ctx) (a b : Ty) : CtxHasType ts (const ts a b) (a :-> b :-> a) :=
+  CtxHasType.CLam (fun x =>
+    CtxHasType.CLam (fun _ =>
+      CtxHasType.CVar (Snoc Refl) x))
+
+def const' : STLCCtx := const Ctx.Empty Unit Unit
+
+def const'Typed : CtxHasType Ctx.Empty const' (Unit :-> Unit :-> Unit) :=
+  constTyped Ctx.Empty Unit Unit
 
 #eval showSTLCCtx const'
 #eval unembed const'
-#eval showSTLCCtx (contextualise (unembedTyped const'))
-#eval unembed (contextualise (unembedTyped const'))
+#eval showSTLCCtx (contextualise (unembedTyped const'Typed))
+#eval unembed (contextualise (unembedTyped const'Typed))
 
-def flipConst : STLCCtx ts (a :-> b :-> b)
-  := CLam (fun _ => CLam (fun y => CVar y))
-def flipConst' := @flipConst Ctx.Empty Unit Unit
+def flipConst (ts : Ctx) (a b : Ty) : STLCCtx :=
+  @CLam ts a (fun _ =>
+    @CLam (ts :/: a) b (fun y =>
+      @CVar ((ts :/: a) :/: b) ((ts :/: a) :/: b) b Refl y))
+
+def flipConstTyped (ts : Ctx) (a b : Ty) : CtxHasType ts (flipConst ts a b) (a :-> b :-> b) :=
+  CtxHasType.CLam (fun _ =>
+    CtxHasType.CLam (fun y =>
+      CtxHasType.CVar Refl y))
+
+def flipConst' : STLCCtx := flipConst Ctx.Empty Unit Unit
+
+def flipConst'Typed : CtxHasType Ctx.Empty flipConst' (Unit :-> Unit :-> Unit) :=
+  flipConstTyped Ctx.Empty Unit Unit
 
 #check flipConst
 #eval showSTLCCtx flipConst'
 #eval unembed flipConst'
-#eval showSTLCCtx (contextualise (unembedTyped flipConst'))
-#eval unembed (contextualise (unembedTyped flipConst'))
+#eval showSTLCCtx (contextualise (unembedTyped flipConst'Typed))
+#eval unembed (contextualise (unembedTyped flipConst'Typed))
 
-def const5 : STLCCtx ts (a :-> b :-> c :-> d :-> e :-> a)
-  := CLam (fun x1 => CLam (fun _ => CLam (fun _ => CLam (fun _ => CLam (fun _ => CVar x1)))))
-def const5' := @const5 Ctx.Empty Unit Unit Unit Unit Unit
+def const5 (ts : Ctx) (a b c d e : Ty) : STLCCtx :=
+  @CLam ts a (fun x1 =>
+    @CLam (ts :/: a) b (fun _ =>
+      @CLam ((ts :/: a) :/: b) c (fun _ =>
+        @CLam (((ts :/: a) :/: b) :/: c) d (fun _ =>
+          @CLam ((((ts :/: a) :/: b) :/: c) :/: d) e (fun _ =>
+            @CVar (ts :/: a) (((((ts :/: a) :/: b) :/: c) :/: d) :/: e) a (Snoc (Snoc (Snoc (Snoc Refl)))) x1)))))
+
+def const5Typed (ts : Ctx) (a b c d e : Ty) : CtxHasType ts (const5 ts a b c d e) (a :-> b :-> c :-> d :-> e :-> a) :=
+  CtxHasType.CLam (fun x1 =>
+    CtxHasType.CLam (fun _ =>
+      CtxHasType.CLam (fun _ =>
+        CtxHasType.CLam (fun _ =>
+          CtxHasType.CLam (fun _ =>
+            CtxHasType.CVar (Snoc (Snoc (Snoc (Snoc Refl)))) x1)))))
+
+def const5' : STLCCtx := const5 Ctx.Empty Unit Unit Unit Unit Unit
+
+def const5'Typed : CtxHasType Ctx.Empty const5' (Unit :-> Unit :-> Unit :-> Unit :-> Unit :-> Unit) :=
+  const5Typed Ctx.Empty Unit Unit Unit Unit Unit
 
 #eval showSTLCCtx const5'
 #eval unembed const5'
-#eval showSTLCCtx (contextualise (unembedTyped const5'))
-#eval unembed (contextualise (unembedTyped const5'))
+#eval showSTLCCtx (contextualise (unembedTyped const5'Typed))
+#eval unembed (contextualise (unembedTyped const5'Typed))
 
-example {ts : Ctx} {a : Ty}
-  : @CLam ts a a (fun x => CVar x) =  @CLam ts a a (fun y => CVar y) := by
+example {ts : Ctx} {a : Ty} :
+    idSTLC ts a = idSTLC ts a := by
   rfl
 
-example {ts : Ctx} {a : Ty}
-  : contextualise (HasType.Lambda (HasType.Var Lookup.Top)) = @CLam ts a a (fun y => CVar y) := by
-  simp [contextualise, toCVar, fromLookup, fromVar]
+example {ts : Ctx} {a : Ty} :
+    contextualise (@HasType.Lambda ts a (STLC.Var Index.Top) a
+      (@HasType.Var (ts :/: a) Index.Top a (@Lookup.Top ts a))) = idSTLC ts a := by
+  simp [contextualise, idSTLC, fromLookup, fromVar, varTop]
   funext x
   cases x
   rfl
