Docs/ContextualEmbedding/__CEFnExample.lean
@@ -1,0 +1,12 @@
+import «ContextualEmbedding».CE
+
+namespace ContextualEmbedding.CE
+
+open STLCCtx
+
+def binaryReturnsFirst : STLCCtx ts (a :-> b :-> a) :=
+  CLam (fun x => CLam (fun _y => CVar x))
+
+#check binaryReturnsFirst
+
+end ContextualEmbedding.CE
