Docs/ContextualEmbedding/package.lean
@@ -1,4 +1,6 @@
 import «ContextualEmbedding».CE
+import «ContextualEmbedding».CEBinaryFunctionExample
+import «ContextualEmbedding».CEEval
 import «ContextualEmbedding».CEExtrinsic
 import «ContextualEmbedding».CELeveledUpSTLC
 import «ContextualEmbedding».CELeveledUpLinear
